src/program_logic/recovery_weakestpre.v
@@ -23,7 +23,7 @@ Definition wpr_pre `{perennialG Λ CS T Σ} (s : stuckness) (k: nat)
   (invG Σ -d> pbundleG T Σ -d> iPropO Σ) -d>
   (invG Σ -d> pbundleG T Σ -d> val Λ -d> iPropO Σ) -d> iPropO Σ :=
   λ H1 H2 t E e rec Φ Φinv Φr,
-  (WPC e @ s ; k; E ; ∅
+  (WPC e @ s ; k; E ; E
      {{ Φ }}
      {{ ∀ σ σ' (HC: crash_prim_step CS σ σ') κs n,
         state_interp σ κs n ={∅}=∗  ▷ ∀ H1 H2, NC ={⊤}=∗ ∃ t, state_interp σ' κs 0 ∗ (Φinv H1 t ∧ wpr H1 H2 t E rec rec (λ v, Φr H1 t v) Φinv Φr) ∗ NC}})%I.
@@ -85,20 +85,21 @@ Qed.
 
 (* To prove a recovery wp for e with rec, it suffices to prove a crash wp for e,
    where the crash condition implies the precondition for a crash wp for rec *)
-Lemma idempotence_wpr s k E e rec Φx Φinv Φrx Φcx Hi Hc t:
-  ((WPC e @ s ; k ; E ; ∅ {{ Φx t }} {{ Φcx t }}) -∗
+Lemma idempotence_wpr s k E1 E2 e rec Φx Φinv Φrx Φcx Hi Hc t:
+  E2 ⊆ E1 →
+  ((WPC e @ s ; k ; E1 ; E2 {{ Φx t }} {{ Φcx t }}) -∗
    (□ ∀ (H: invG Σ) (Hc: crashG Σ) (t: pbundleG T Σ) σ σ' (HC: crash_prim_step CS σ σ') κs n,
         Φcx t -∗ state_interp σ κs n ={∅}=∗
-        ▷ ∀ H' (Hc': crashG Σ), NC ={⊤}=∗ ∃ t', state_interp σ' κs 0 ∗ (Φinv H' t' ∧ WPC rec @ s ; k; E ; ∅ {{ Φrx H' t' }} {{ Φcx t' }}) ∗ NC) -∗
-    wpr s k Hi Hc t E e rec (Φx t) Φinv Φrx)%I.
+        ▷ ∀ H' (Hc': crashG Σ), NC ={⊤}=∗ ∃ t', state_interp σ' κs 0 ∗ (Φinv H' t' ∧ WPC rec @ s ; k; E1 ; E2 {{ Φrx H' t' }} {{ Φcx t' }}) ∗ NC) -∗
+    wpr s k Hi Hc t E1 e rec (Φx t) Φinv Φrx)%I.
 Proof.
-  iLöb as "IH" forall (E e Hi Hc t Φx).
-  iIntros "He #Hidemp".
+  iLöb as "IH" forall (E1 E2 e Hi Hc t Φx).
+  iIntros (?) "He #Hidemp".
   rewrite wpr_unfold. rewrite /wpr_pre.
-  iApply (wpc_strong_mono' with "He"); [ auto | auto | auto | set_solver+ | ].
+  iApply (wpc_strong_mono' with "He"); [ auto | auto | auto | set_solver | ].
   iSplit; first auto. iIntros "Hcx".
-  rewrite difference_diag_L.
-  iModIntro.
+  iApply @fupd_mask_weaken.
+  { set_solver +. }
   iIntros. iMod ("Hidemp" with "[ ] [$] [$]") as "H".
   { eauto. }
   iModIntro. iNext. iIntros (Hi' Hc') "HNC". iMod ("H" $! Hi' Hc' with "[$]") as (t') "(?&Hc&HNC)".
@@ -106,7 +107,7 @@ Proof.
   iSplit.
   { iDestruct "Hc" as "($&_)". }
   iDestruct "Hc" as "(_&Hc)".
-  iApply ("IH" $! E rec Hi' Hc' t' (λ t v, Φrx Hi' t v)%I with "[Hc]").
+  iApply ("IH" $! E1 E2 rec Hi' Hc' t' (λ t v, Φrx Hi' t v)%I with "[//] [Hc]").
   { iApply (wpc_strong_mono' with "Hc"); rewrite ?difference_diag_L; auto. }
   eauto.
 Qed.
